fixed the 0/1 confusion. The types (classes) Zero and One are now NOT definitionally equal. Typeclass resolution still has some problems: 1) a ring contains 2 semigroups. When using lemmas about semigroups for rings, there are ambiguous ways to form a semigroup. The other instances like join_is_sg_op (join is a semigrou operator) also complicate the resolution. Perhaps the resolution algorithm should first try to resolve the SemiGroup instance before try to find out the semigroup operator (SgOp). Is there a way to express such strategies in Coq? Would such strategies be really more robust?
2) Because Plus A is now Not definitionally equal to A -> A-> A, some extra folding is needed to apply the lemmas from abstract algebra. Perhaps this can be automated in
a predictable way?

src/interfaces/canonical_names.v
@@ -104,13 +104,13 @@ Class SgOp A := sg_op: A → A → A.
 Class MonUnit A := mon_unit: A.
 Class Plus A := {plus: A → A → A}.
 Class Mult A := {mult: A → A → A}.
-Class One A := one: A.
-Class Zero A := zero: A.
+Class One A := { one: A }.
+Class Zero A := { zero: A}.
 Class Negate A := negate: A → A.
 Class DecRecip A := dec_recip: A → A.
 Definition ApartZero R `{Zero R} `{Apart R} := sig (≶ zero).
 Class Recip A `{Apart A} `{Zero A} := recip: ApartZero A → A.
-Typeclasses Transparent SgOp MonUnit  Zero One Negate.
+Typeclasses Transparent SgOp MonUnit Negate.
 
 Class Meet A := meet: A → A → A.
 Class Join A := join: A → A → A.
@@ -158,15 +158,6 @@ Instance: Params (@contains) 3.
 Instance: Params (@singleton) 3.
 Instance: Params (@difference) 2.
 
-Instance plus_is_sg_op `{f : Plus A} : SgOp A.
-  destruct f. exact plus0.
-Defined.
-Instance mult_is_sg_op `{f : Mult A} : SgOp A.
-  destruct f. exact mult0.
-Defined.
-
-Instance one_is_mon_unit `{c : One A} : MonUnit A := c.
-Instance zero_is_mon_unit `{c : Zero A} : MonUnit A := c.
 Instance meet_is_sg_op `{f : Meet A} : SgOp A := f.
 Instance join_is_sg_op `{f : Join A} : SgOp A := f.
 Instance top_is_mon_unit `{s : Top A} : MonUnit A := s.
